While rule with variant decoration
git-svn-id: orca@515

C-verifier/src/Midend-IVL/Isabelle-UTP-Extended/theories/Abrupt/utp_abrupt_designs.thy
@@ -1,6 +1,6 @@
 theory utp_abrupt_designs
-imports   "../../../Isabelle-UTP/theories/utp_designs"
-          "../../hoare/AlgebraicLaws/Rel&Des/Algebraic_Laws_aux"
+imports   "../Design/utp_designs_more"
+
 begin
 subsection {*Sequential C-program alphabet*}
 
@@ -128,28 +128,13 @@ subsection {* Reactive lemmas *}
 
 subsection{*Healthiness conditions*}
 
-text {*Programs in abrupt state do not progress*}
-definition C3_abr_def [upred_defs]: 
-  "C3_abr(P) = (P \<triangleleft> \<not>$abrupt \<triangleright> II)"
-
+text {*Programs in abrupt state do not progress*}   
 abbreviation
- "Simpl\<^sub>A\<^sub>B\<^sub>R P \<equiv> C3_abr(\<lceil>true\<rceil>\<^sub>A\<^sub>B\<^sub>R \<turnstile> (P))"
+ "Simpl\<^sub>A\<^sub>B\<^sub>R P \<equiv> ((\<not>$abrupt \<turnstile> P) \<squnion> ($abrupt  \<turnstile> II))"
 
 subsection{*Control flow statements*}
 
-text
-{*
-  We introduce the known control-flow statements for C. Our semantics is restricted
-  to @{const C3_abr}. In other words It assumes:
-  \begin{itemize}   
-    \<^item>  If we start the execution of a program ie, @{term "$ok"}, from an initial stable state ie,
-       @{term "\<not>($abrupt)"},   
-    \<^item>  the program can terminates and has a final state ie,@{term "$ok\<acute>"},
-    \<^item>  the final state is a normal state if it terminates and the result of execution is 
-       @{term "\<not>$abrupt"},
-  \end{itemize}
-  Thus it capture Simpl semantics.
-*}
+text {**}
 
 definition skip_abr :: "('\<alpha>) hrel_cpa" ("SKIP\<^sub>A\<^sub>B\<^sub>R")
 where [urel_defs]:
@@ -159,9 +144,9 @@ subsection{*THROW*}
 
 definition throw_abr :: "('\<alpha>) hrel_cpa" ("THROW\<^sub>A\<^sub>B\<^sub>R")
 where [urel_defs]: 
-  "THROW\<^sub>A\<^sub>B\<^sub>R = ((\<not>$abrupt)\<turnstile> ($abrupt\<acute> \<and> \<lceil>II\<rceil>\<^sub>A\<^sub>B\<^sub>R))"
+  "THROW\<^sub>A\<^sub>B\<^sub>R = Simpl\<^sub>A\<^sub>B\<^sub>R($abrupt\<acute> \<and> \<lceil>II\<rceil>\<^sub>A\<^sub>B\<^sub>R)"
 
-definition assigns_abr :: " '\<alpha> usubst \<Rightarrow> ('\<alpha>) hrel_cpa" ("\<langle>_\<rangle>\<^sub>A\<^sub>B\<^sub>R")
+definition assigns_abr :: "'\<alpha> usubst \<Rightarrow> ('\<alpha>) hrel_cpa" ("\<langle>_\<rangle>\<^sub>A\<^sub>B\<^sub>R")
 where [urel_defs]: 
   "assigns_abr \<sigma> = Simpl\<^sub>A\<^sub>B\<^sub>R (\<not>$abrupt\<acute> \<and> \<lceil>\<langle>\<sigma>\<rangle>\<^sub>a\<rceil>\<^sub>A\<^sub>B\<^sub>R)"
 
@@ -197,8 +182,8 @@ subsection{*Loops*}
 
 purge_notation while ("while\<^sup>\<top> _ do _ od")
 
-definition While :: "'\<alpha> cond \<Rightarrow> ('\<alpha>) hrel_cpa \<Rightarrow> ('\<alpha>) hrel_cpa" ("while\<^sup>\<top> _ do _ od") where
-"While b C = (\<nu> X \<bullet> bif b then (C ;; X) else SKIP\<^sub>A\<^sub>B\<^sub>R eif)"
+definition While_abr_top :: "'\<alpha> cond \<Rightarrow> ('\<alpha>) hrel_cpa \<Rightarrow> ('\<alpha>) hrel_cpa" ("while\<^sup>\<top> _ do _ od") where
+"While b C = (\<nu>\<^sub>D X \<bullet> bif b then (C ;; X) else SKIP\<^sub>A\<^sub>B\<^sub>R eif)"
 
 purge_notation while_top ("while _ do _ od")
 
