C-verifier/src/Midend-IVL/Isabelle-UTP-Extended/utp/utp_sp.thy
@@ -1,5 +1,5 @@
 theory utp_sp
-imports "../hoare/HoareLogic/PartialCorrectness/utp_hoare"
+imports "../../Isabelle-UTP/utp/utp_wp"
     
 begin
 
@@ -42,7 +42,11 @@ lemma "\<lbrace>p\<rbrace>C\<lbrace>p sp C\<rbrace>\<^sub>u"
   by rel_blast
 
 theorem sp_eq_intro: "\<lbrakk>\<And>r. r sp P = r sp Q\<rbrakk> \<Longrightarrow> P = Q"
-  by (rel_auto robust, fastforce+)    
-
+  by (rel_auto robust, fastforce+)  
+    
+lemma wp_sp_sym:
+  "`prog wp (true sp prog)`"
+  by rel_auto
+    
 end  
   
